More limpeza

LeanProjeto2/SHFunctInterp.lean
@@ -45,160 +45,56 @@ The function 'Recreate' transforms a tuple such as (a,b,A_SH) into the formula �
 
 -- É PRECISO ACRESCENTAR ISFULLYBASE, aka que temos necessariamente uma fórmula sem ∀ e sem ∃ na matriz
 
-#check isBase
 
-def Formula.components : Formula → (Finset String × Finset String × Formula)
+-- OBS: Components é para termos as components de um interpretação!
+-- Só se pode usar quando ja estiver com ∀a ∃b ...
+def Formula.components : Formula → (List String × List String × Formula)
 | unbForall x A =>
     let (a, b, rest) := A.components
-    ({x} ∪ a, b, rest)
+    ([x] ∪ a, b, rest)
 | not (unbForall x A) =>
     let (a, b, rest) := A.components
-    (a, {x} ∪ b, rest)
+    (b, [x] ∪ a, not rest)
+| not (not A) =>
+    -- This handles the double negation case
+    A.components
 | not A =>
     let (a, b, rest) := A.components
-    (a, b, not rest)
---| bForall x t A =>
---    let (a, b, rest) := A.components
---    (a, {x} ∪ b, bForall x t rest)
+    (b, a, not rest)
 | or A1 A2 =>
     let (a1, b1, r1) := A1.components
     let (a2, b2, r2) := A2.components
     (a1 ∪ a2, b1 ∪ b2, or r1 r2)
-| A => ({}, {}, A)
--- Reunião: daria se calhar para pôr aqui um not e forall
--- Só se pode usar quando ja estiver com ∀a ∃b
-
-def Formula.components2 : Formula → (List String × List String × Formula)
-| unbForall x A =>
-    let (a, b, rest) := A.components2
-    ({x} ∪ a, b, rest)
-| not (unbForall x A) =>
-    let (a, b, rest) := A.components2
-    (a, {x} ∪ b, rest)
-| not A =>
-    let (a, b, rest) := A.components2
-    (a, b, not rest)
---| bForall x t A =>
---    let (a, b, rest) := A.components
---    (a, {x} ∪ b, bForall x t rest)
-| or A1 A2 =>
-    let (a1, b1, r1) := A1.components2
-    let (a2, b2, r2) := A2.components2
-    (a1 ∪ a2, b1 ∪ b2, or r1 r2)
-| A => ({}, {}, A)
-
-
-def Formula.components5 : Formula → (List String × List String × Formula)
-| unbForall x A =>
-    let (a, b, rest) := A.components5
-    ({x} ∪ a, b, rest)
-| not (unbForall x A) =>
-    let (a, b, rest) := A.components5
-    (b, {x} ∪ a, not rest)
-| not (not A) =>
-    -- This handles the double negation case
-    A.components5
-| not A =>
-    let (a, b, rest) := A.components5
-    (b, a, not rest)
-| or A1 A2 =>
-    let (a1, b1, r1) := A1.components5
-    let (a2, b2, r2) := A2.components5
-    (a1 ∪ a2, b1 ∪ b2, or r1 r2)
 | bForall x t A =>
-    let (a, b, rest) := A.components5
-    (a, {x} ∪ b, bForall x t rest)
+    let (a, b, rest) := A.components
+    (a, b, bForall x t rest)
+    --(a, [x] ∪ b, bForall x t rest)
 | A => ([], [], A)
 
-def Formula.dia : Formula → List String → List String → Formula → Prop
-| F, u, e, f => F.components5 = (u, e, f)
-
-
-example (A:Formula) : A.dia u e f1 → u == ["x"] := by sorry
-
-example (A:Formula) (h: isBase A) : A.components5 = (∅,∅,A) := by
-  sorry
 
 -- -------
 -- Example to use components:
 -- -------
 
-def formula_teste (A:Formula) : Formula := (∀₁₁ "x" (∃₁₁ "y" (∃₁₁ "z" (¬₁A))))
-#eval (formula_teste (Formula.rel "R" [var_x,var_y])).components      -- Output: ({x}, {y, z}, ¬₁R(x,y)) --> CAN I ADD SIMP??
-#eval components (∀₁₁ "x" (¬₁(∀₁₁ "y" (rel "P" [var_x, var_y]))))     -- Output: ({x}, {y, z}, ¬₁R(x,y))
-#eval components (∀₁₁ "x" ((∃₁₁ "y" (¬₁(rel "P" [var_x, var_y])))))   -- Output: ({x}, {y, z}, ¬₁R(x,y))
+def ex_formula_comp1 (A:Formula) : Formula := (∀₁₁ "x" (∃₁₁ "y" (∃₁₁ "z" (¬₁A))))
+#eval (ex_formula_comp1 (Formula.rel "R" [var_x,var_y])).components               -- Output: ([x], [y, z], ¬₁R(x,y))
+#eval components (∀₁₁ "x" (¬₁(∀₁₁ "y" (rel "P" [var_x, var_y]))))                 -- Output: ([x], [y, z], ¬₁R(x,y))
+#eval components (∀₁₁ "x" ((∃₁₁ "y" (¬₁(rel "P" [var_x, var_y])))))               -- Output: ([x], [y, z], ¬₁R(x,y))
 
-def exampleFormula : Formula :=
-  b∀₁₁ "x" (Term.var "t") (¬₁ (∀₁₁ "y" (Formula.rel "R" [])))
-#eval exampleFormula.components       -- Output dá ({}, {x,y}, ∀x∈t R[]) --> WRONG
+def ex_formula_comp2 : Formula :=
+  ∀₁ ["x"] (¬₁ (b∀₁₁ "y" (Term.var "t") (Formula.rel "R" [var "y"])))
+#eval ex_formula_comp2.components                                                 -- Output: (["x"], [], ∀y∈t R[y])
 
-
-noncomputable def Recreate : (Finset String × Finset String × Formula) → Formula
-| (a, b, rest) => -- Assim já ficamos com (x,y,F)
-  -- Negações dentro do b
-                let neg := List.foldl (fun f x => .unbForall x (.not f)) rest (b.val.toList : List String)
-  -- unbForall dentro do a
-                List.foldl (fun f x => .unbForall x f) neg (a.val.toList : List String)
--- TBD (Reunião): dá para acrescentar aqui que rest is always base?
---   -> Não vai ser consequência direta de acrescentar isBase como hipotese em components?
-
-def Recreate2 : (List String × List String × Formula) → Formula
-| (a, b, rest) =>
-  -- Negações dentro do b
-  let neg := List.foldl (fun f x => .unbForall x (.not f)) rest b
-  -- unbForall dentro do a
-  List.foldl (fun f x => Formula.unbForall x f) neg a
-
-def Recreate22 : (List String × List String × Formula) → Formula
-| (a, b, rest) =>
-  -- Negações dentro do b
-  let neg := List.foldl (fun f x => .unbForall x (.not f)) rest b
-  -- unbForall dentro do a
-  List.foldl (fun f x => Formula.unbForall x f) neg a
-
-def Recreate3 : (List String × List String × Formula) → Formula
-| (a, b, rest) =>
-  -- Apply universal quantifiers first
-  let apply_unbForall := List.foldl (fun f x => Formula.unbForall x f) rest a
-  -- Apply negations to existential quantifiers
-  let apply_negations := List.foldl (fun f x => Formula.not (Formula.unbForall x (Formula.not f))) apply_unbForall b
-  apply_negations
-
-def Recreate4 : (List String × List String × Formula) → Formula
-| (a, b, rest) =>
-  -- Apply universal quantifiers from `a` first
-  let with_unbForalls := List.foldr (fun x f => Formula.unbForall x f) rest a
-  -- Apply negations to existential quantifiers from `b` and wrap in the universal quantifiers
-  let apply_negations := List.foldl (fun f x => Formula.not (Formula.unbForall x (Formula.not f))) with_unbForalls b
-  apply_negations
-
-def Recreate5 : (List String × List String × Formula) → Formula
-| (a, b, rest) =>
-  -- Apply universal quantifiers from `a` in the order they appear
-  let with_unbForalls := List.foldr (fun x f => Formula.unbForall x f) rest a
-  -- Apply existential quantifiers from `b` in reverse order with negations
-  List.foldl (fun f x => Formula.not (Formula.unbForall x (Formula.not f))) with_unbForalls b
-
-def Recreate6 : (List String × List String × Formula) → Formula
-| (a, b, rest) =>
-  -- Apply universal quantifiers from `a` in the order they appear
-  let with_unbForalls := List.foldr (fun x f => Formula.unbForall x f) rest a
-  -- Apply existential quantifiers from `b` in reverse order with negations
-  List.foldr (fun x f => (Formula.unbForall x f)) with_unbForalls b
-
-def Recreate7 : (List String × List String × Formula) → Formula
-| (a, b, rest) =>
-  -- Apply universal quantifiers from `a` in the order they appear
-  let with_existentials := List.foldr (fun x f => .not (Formula.unbForall x (.not f))) rest b
-  -- Apply existential quantifiers from `b` in reverse order with negations
-  List.foldr (fun x f => (Formula.unbForall x f)) with_existentials a
+-- --------
+-- Recreate
+-- --------
 
 @[simp]
-def Recreate8 : (List String × List String × Formula) → Formula
+def RecreateSimp : (List String × List String × Formula) → Formula
 | (a, b, rest) => ∀₁ a (∃₁ b rest)
 
 @[simp]
-def RecreateEmpty : (List String × List String × Formula) → Formula
+def Recreate : (List String × List String × Formula) → Formula
 | ([], [], rest) => rest
 | (a, [], rest) => ∀₁ a rest
 | ([], b, rest) => ∃₁ b rest
@@ -215,116 +111,38 @@ Here we will represent an interpretation A^SH such as ∀a∃b A_SH(a,b) as
               ( SH_int upperSH ( Recreate (univ_var,exist_var,lowerSH) ) )
 -/
 
-
--- TBD (Reunião): variaveis disjuntas -> Finset já tem disjunto
---                make List α to Finset -> List.toFinset _
--- a∪b∪c∪d : Finset     -> ver Disjoint a b c d
-inductive SH_int : Formula → Formula → Prop
-| base : (h : isFullyBase A) → (SH_int A (Recreate ({},{},A)))
-| disj : SH_int A AuSH →
-         SH_int B BuSH →
-         AuSH.components = (a,b,A_SH) →                                     -- A^SH = ∀a ∃b A_SH(a,b)
-         BuSH.components = (c,d,B_SH) →                                     -- B^SH = ∀c ∃d B_SH(c,d)
-         --({a,b} ⊆ A.allvars) →                                            -- TO DO: precisamos?
-         --({c,d} ⊆ B.allvars) →                                            -- TO DO: dizer lista não tem conjuntos repetidos
-         (hA : isFullyBase A_SH) →
-         (hB : isFullyBase B_SH) →
-         (SH_int (A∨₁B) (Recreate (a∪c,b∪d,(A_SH ∨₁ B_SH))))                -- (A∨B)^SH = ∀a,c ∃b,d [ A_SH(a,b) ∨ B_SH(c,d) ]
-| neg {f a':String}:
-        -- ({a,b} ⊆ A.allvars) →
-        SH_int A AuSH →
-        AuSH.components = (a,b,A_SH) →                                     -- A^SH = ∀a ∃b A_SH(a,b)
-        (hA : isFullyBase A_SH) →
-        (SH_int (¬₁A) (Recreate (b,b,A_SH)))--(TermTupleApp (makeTuple [Term.var f]) a)))) --→  -- TODO: apagar porque foi batota
-        --(SH_int (¬₁A) (Recreate ({f},{a'},(b∃₁ a.toList (Term.var a') (¬₁(substitution_formula b.toList ((Term.var f)·(Term.var a)) A_SH))))))
-        --(SH_int (¬₁A) (Recreate ({f},{a'},(b∃₁ a.toList (Term.var a') A))))
-        --(SH_int (¬₁A) (Recreate ({f},{a'},(b∃₁ a.toList (Term.var a') (¬₁(substitution_formula b.toList ((Term.var f)·(Term.var a)) A_SH))))))      -- TO DO / Problema: problema: o bE₁ devia então aceitar Finset String :'(
-        --((SH_int (¬₁A) (V₁ f (E₁ a' (bE₁ a (Term.var (a')) (¬₁(substitution_formula b ((Term.var f)·(Term.var a)) A_SH)))))))         -- (¬A)^SH = ∀f ∃a' [ ∃a∈a' ¬A_SH(a,fa) ]
-        --(SH_int2 (¬₁A) (Recreate2 (b,b,(bForallTuple2 a (ls_lt a') A_SH))))--(TermTupleApp (makeTuple [Term.var f]) a)))) --→  -- TODO: apagar porque foi batota
-        --(SH_int2 (¬₁A) (Recreate2 (f,a',(b∃₁ a (Term.var a') A_SH))))
-
-| unbForall : SH_int A AuSH →
-              AuSH.components = (a,b,A_SH) →                                -- A^SH = ∀a ∃b A_SH(a,b)
-              --({x,a,b} ⊆ A.allvars) →
-              --(SH_int A (V₁ a (E₁ b A_SH))) →                             -- A^SH = ∀a ∃b A_SH(a,b)
-              (hA : isFullyBase A_SH) →
-              (SH_int (∀₁₁ x A) (Recreate (a∪{x},b,A_SH)))                  -- (∀x A)^SH = ∀x,a ∃b [ A_SH(x,a,b) ]
-| bForall : SH_int A AuSH →
-            AuSH.components = (a,b,A_SH) →                                  -- A^SH = ∀a ∃b A_SH(a,b)
-            (hA : isFullyBase A_SH) →
-            (SH_int (b∀₁ x t A) (Recreate (a,b,(b∀₁ x t A_SH))))            -- (∀x∈t A(x))^SH = ∀a ∃b [ ∀x∈t A_SH(x,a,b) ]
-            --({x,a,b} ⊆ A.allvars) →
-            --(h : x ∉ t.freevars)
-
-
 -- TO DO (eu): a tirar este Teste e fazer um melhor
 def Teste (a b : String) (f : Term) (A_SH : Formula): Formula := substitution_formula b (f·(Term.var a)) A_SH
-
-example (A:Formula) (H : isBase A) : isBase (b∃₁₁ x t A) := by
-  exact bExists_base x t H
-
--- PRECISAMOS DE COMPONENTS?? NAO PODE SER SO UM TUPLO QUALQUER QUE DEPOIS USAMOS AQUI??? HELP
--- COMPONENTS SO USAR PARA COMPONENTS DE INTERPRETACOES
 
 inductive SH_int2 : Formula → Formula → Prop
 | base : (h : isBase A) → (SH_int2 A A)
 | disj : SH_int2 A AuSH →
          SH_int2 B BuSH →
-         AuSH.components5 = (a,b,A_SH) →                                     -- A^SH = ∀a ∃b A_SH(a,b)
-         BuSH.components5 = (c,d,B_SH) →                                     -- B^SH = ∀c ∃d B_SH(c,d)
-         --({a,b} ⊆ A.allvars) →                                            -- TO DO: precisamos?
-         --({c,d} ⊆ B.allvars) →                                            -- TO DO: dizer lista não tem conjuntos repetidos
-         --(hA : isBase A_SH) →
-         --(hB : isBase B_SH) →
-         (SH_int2 (A∨₁B) (RecreateEmpty (a∪c,b∪d,(A_SH ∨₁ B_SH))))                -- (A∨B)^SH = ∀a,c ∃b,d [ A_SH(a,b) ∨ B_SH(c,d) ]
+         AuSH.components = (a,b,A_SH) →                                     -- A^SH = ∀a ∃b A_SH(a,b)
+         BuSH.components = (c,d,B_SH) →                                     -- B^SH = ∀c ∃d B_SH(c,d)
+         (SH_int2 (A∨₁B) (Recreate (a∪c,b∪d,(A_SH ∨₁ B_SH))))           -- (A∨B)^SH = ∀a,c ∃b,d [ A_SH(a,b) ∨ B_SH(c,d) ]
 | neg {f a': List String}:
-        -- ({a,b} ⊆ A.allvars) →
         SH_int2 A AuSH →
-        (a,b,A_SH) = AuSH.components5 →                                    -- A^SH = ∀a ∃b A_SH(a,b)
-        --(hA : isBase A_SH) →
-        (SH_int2 (¬₁A) (RecreateEmpty (f,a',(bForallTuple2 a (ls_lt a') (¬₁(A_SH.subst (HashMap.ofList  (b.zip ((f.tt)⊙(a.tt))))))))))
+        (a,b,A_SH) = AuSH.components →                                      -- A^SH = ∀a ∃b A_SH(a,b)
+        (SH_int2 (¬₁A) (Recreate (f,a',(bForallTuple2 a (ls_lt a') (¬₁(A_SH.subst (HashMap.ofList  (b.zip ((f.tt)⊙(a.tt))))))))))
 | unbForall : SH_int2 A AuSH →
-              AuSH.components5 = (a,b,A_SH) →                                -- A^SH = ∀a ∃b A_SH(a,b)
-              --({x,a,b} ⊆ A.allvars) →
-              --(SH_int A (V₁ a (E₁ b A_SH))) →                             -- A^SH = ∀a ∃b A_SH(a,b)
-              --(hA : isBase A_SH) →
-              (SH_int2 (∀₁₁ x A) (RecreateEmpty (a∪{x},b,A_SH)))                  -- (∀x A)^SH = ∀x,a ∃b [ A_SH(x,a,b) ]
+              AuSH.components = (a,b,A_SH) →                                -- A^SH = ∀a ∃b A_SH(a,b)
+              (SH_int2 (∀₁₁ x A) (Recreate (a∪{x},b,A_SH)))             -- (∀x A)^SH = ∀x,a ∃b [ A_SH(x,a,b) ]
 | bForall : SH_int2 A AuSH →
-            AuSH.components5 = (a,b,A_SH) →                                  -- A^SH = ∀a ∃b A_SH(a,b)
-            --(hA : isBase A_SH) →
-            (SH_int2 (b∀₁ x t A) (RecreateEmpty (a,b,(b∀₁ x t A_SH))))            -- (∀x∈t A(x))^SH = ∀a ∃b [ ∀x∈t A_SH(x,a,b) ]
-            --({x,a,b} ⊆ A.allvars) →
-            --(h : x ∉ t.freevars)
+            AuSH.components = (a,b,A_SH) →                                  -- A^SH = ∀a ∃b A_SH(a,b)
+            (SH_int2 (b∀₁ x t A) (Recreate (a,b,(b∀₁ x t A_SH))))       -- (∀x∈t A(x))^SH = ∀a ∃b [ ∀x∈t A_SH(x,a,b) ]
 
-def Formula.components6 : Formula → (List String × List String × Formula)
-| unbForall x A =>
-    let (a, b, rest) := A.components5
-    ({x} ∪ a, b, rest)
-| not (unbForall x A) =>
-    let (a, b, rest) := A.components5
-    (b, {x} ∪ a, not rest)
-| not (not A) =>
-    -- This handles the double negation case
-    A.components5
-| not A =>
-    let (a, b, rest) := A.components5
-    (b, a, not rest)
-| or A1 A2 =>
-    let (a1, b1, r1) := A1.components5
-    let (a2, b2, r2) := A2.components5
-    (a1 ∪ a2, b1 ∪ b2, or r1 r2)
-| bForall x t A =>
-    let (a, b, rest) := A.components5
-    (a, {x} ∪ b, bForall x t rest)
-| A => ([], [], A)
-
-@[simp]
-def DoubleNeg (A:Formula) := ((¬₁(¬₁ A)) = A)
+--(hA : isBase A_SH) →
+-- ({a,b} ⊆ A.allvars) →
+--({x,a,b} ⊆ A.allvars) →
+--(h : x ∉ t.freevars)
 
 
 
-example (h1: SH_int2 A AuSH) (h2 : AuSH.components5 = (a,b,A_SH))
-        (h3: SH_int2 (∀₁₁ x A) interp) : interp.components5 = ([x]∪a,b,A_SH) := by
+
+
+example (h1: SH_int2 A AuSH) (h2 : AuSH.components = (a,b,A_SH))
+        (h3: SH_int2 (∀₁₁ x A) interp) : interp.components = ([x]∪a,b,A_SH) := by
   let H := @SH_int2.unbForall A AuSH a b A_SH x h1 h2
   sorry
 
@@ -341,6 +159,31 @@ inductive SH_int_comp : Formula → (List String × List String × Formula) → 
 | bForall : SH_int_comp A (a,b,A_SH) →
             (SH_int_comp (b∀₁ x t A) (a,b,(b∀₁ x t A_SH)))            -- (∀x∈t A(x))^SH = ∀a ∃b [ ∀x∈t A_SH(x,a,b) ]
 
+--({a,b} ⊆ A.allvars) →
+--({c,d} ⊆ B.allvars) →
+--({x,a,b} ⊆ A.allvars) →
+--(h : x ∉ t.freevars)
+
+-- variaveis disjuntas -> Finset já tem disjunto
+-- a∪b∪c∪d : Finset     -> ver Disjoint a b c d
+
+-- ------------------------------------------------------
+
+-- DEFINITION: Interpretation of base formulas is the base formulas themselves
+
+@[simp]
+def baseBase (A:Formula) (hA : isBase A) (hIntA: SH_int2 A AuSH) (hAcomp: AuSH.components = ({},{},A_SH))
+  := A_SH = A
+
+@[simp] -- DEFINITION: If A is base, then the lower SH-formula is equal to A
+def baseBase_comp (A:Formula) (hA : isBase A) (hIntA: SH_int_comp A ([],[],A_SH))
+  := A_SH = A
+
+@[simp] -- DEFINITION: If A is base, then the interpretation of A is equal to A
+def baseBase_rec (A:Formula) (hA : isBase A) (hIntA: SH_int_comp A ([],[],A_SH))
+  := (Recreate ([],[],A_SH)) = A
+
+-- ------------------------------------------------------
 
 inductive SH_int_type : Type
 | mk : List String → List String → Formula → SH_int_type
@@ -367,6 +210,11 @@ def extract_tuple_base {A A_SH: Formula} (hA : isBase A)
   ([], [], A)
 -/
 
+-- --------------------------------------------------------------
+-- EXAMPLE 2.1 (p.38)
+-- Interpretation of (A ∨ (∀x∈t B(x))), with B(x) a base formula.
+-- --------------------------------------------------------------
+
 --#check List.union_nil
 
 lemma List.cons_eq (head:A) (tl1 tl2: List A) : tl1 = tl2 → h :: tl1 = h :: tl2 := by sorry
@@ -377,12 +225,13 @@ lemma List.union_nilTPC (l : List String) (heq : eraseDup l = l) : l ∪ [] = l 
 @[simp]
 lemma List.union_nil (l : List String): l ∪ [] = l := by sorry
 
-
+-- Example teste: (∀₁₁ x A)^SH = ∀ a,x ∃ b A_SH
 example (h: SH_int_comp A (a,b,A_SH)) :
         SH_int_comp (∀₁₁ x A) (a∪[x],b,A_SH) :=
 by
   exact @SH_int_comp.unbForall A a b A_SH x h
 
+-- EXAMPLE 2.1: (A ∨ (∀x∈t B(x)))^SH = ∀a ∃b (A_SH ∨₁ (b∀₁ [x] t B))
 example (A B : Formula) (hA: SH_int_comp A (a,b,A_SH)) (hB : isBase B) :
         SH_int_comp (A ∨₁ (b∀₁ [x] t B)) (a,b,(A_SH ∨₁ (b∀₁ [x] t B))) :=
 by
@@ -394,43 +243,85 @@ by
   rw [Ha,Hb] at H3
   exact H3
 
+-- ---------------------------------------------------------------------
+-- EXAMPLE 2.2 (p.38)
+-- Interpretation of ∀y∈t ¬(∃x A(x) ∧ B(y)).
+-- ---------------------------------------------------------------------
+
+#check ex_2_1_PrimSymb
+
+lemma ex_2_1_PrimSymbb (A B : Formula) (x y : String) (t : Term) : (b∀₁₁ y t (¬₁((∃₁₁ x (¬₁A))∧₁B))) = (b∀₁₁ y t ((∀₁₁ x A)∨₁(¬₁B))) :=
+by
+  rw [DeMorgan_and (∃₁₁ x (¬₁A)) B]
+  unfold unbExists
+  rw [DoubleNeg, DoubleNeg]
+
+-- EXAMPLE 2.1: (∀y∈t ¬(∃x ¬A(x) ∧ B(y)))^SH = ∀a ∃b (A_SH ∨₁ (b∀₁ [x] t B))
+example (A B : Formula)
+        (hA: SH_int_comp A (a,b,A_SH))
+        (hB: SH_int_comp B (c,d,B_SH)) :
+        SH_int_comp (b∀₁₁ y t (¬₁((∃₁₁ x (¬₁ A))∧₁B))) ([x]∪a∪g,b∪c',(b∀₁₁ y t (A_SH ∨₁ (bExistsTuple2 c (c'.tt) (B_SH.subst (HashMap.ofList (d.zip ((g.tt)⊙(c.tt))))))))) :=
+by
+  have H := ex_2_1_PrimSymbb A B y x t
+  --rw [←H]
+  have H1 := @SH_int_comp.unbForall A a b A_SH x hA
+  sorry
+
+
+
+
+
+
+
+
+
+
+
+
+-- --------------------------------------------------------
+-- --------------------------------------------------------
+-- --------------------------------------------------------
 
 -- ------------------------------------------------
 -- COMPUTAR SH INTERPRETATION COM OUTPUT DE FORMULA
 -- ------------------------------------------------
 
-def SH_int_base_rec (A:Formula) (H: isBase A): Formula := (RecreateEmpty ([], [], A))
+def SH_int_base_rec (A:Formula) (H: isBase A): Formula := (Recreate ([], [], A))
 def SH_int_base_comp (A:Formula) (H: isBase A): (List String × List String × Formula) := ([], [], A)
 
 def SH_int_or_rec (A B : Formula)
-  (hIntA: SH_int2 A AuSH) (hAcomp: (a,b,A_SH) = AuSH.components5)
-  (hIntB: SH_int2 B BuSH) (hBcomp: (c,d,B_SH) = BuSH.components5): Formula :=
-  Recreate8 (a∪c, b∪d, (A_SH ∨₁ B_SH))
+  (hIntA: SH_int2 A AuSH) (hAcomp: (a,b,A_SH) = AuSH.components)
+  (hIntB: SH_int2 B BuSH) (hBcomp: (c,d,B_SH) = BuSH.components): Formula :=
+  Recreate (a∪c, b∪d, (A_SH ∨₁ B_SH))
 
 def SH_int_or_comp (A B : Formula)
-  (hIntA: SH_int2 A AuSH) (hAcomp: (a,b,A_SH) = AuSH.components5)
-  (hIntB: SH_int2 B BuSH) (hBcomp: (c,d,B_SH) = BuSH.components5): (List String × List String × Formula) :=
+  (hIntA: SH_int2 A AuSH) (hAcomp: (a,b,A_SH) = AuSH.components)
+  (hIntB: SH_int2 B BuSH) (hBcomp: (c,d,B_SH) = BuSH.components): (List String × List String × Formula) :=
   (a∪c, b∪d, (A_SH ∨₁ B_SH))
 
 def SH_int_unbForall_rec (A : Formula) (x : List String)
-  (hIntA: SH_int2 A AuSH) (hAcomp: (a,b,A_SH) = AuSH.components5): Formula :=
-  Recreate8 (a∪x, b, A_SH)
+  (hIntA: SH_int2 A AuSH) (hAcomp: (a,b,A_SH) = AuSH.components): Formula :=
+  Recreate (a∪x, b, A_SH)
 
 def SH_int_unbForall_comp (A : Formula) (x : List String)
-  (hIntA: SH_int2 A AuSH) (hAcomp: (a,b,A_SH) = AuSH.components5): (List String × List String × Formula) :=
+  (hIntA: SH_int2 A AuSH) (hAcomp: (a,b,A_SH) = AuSH.components): (List String × List String × Formula) :=
   (a∪x, b, A_SH)
 
 def SH_int_bForall_rec (A : Formula) (x : List String) (t : List Term)
-  (hIntA: SH_int2 A AuSH) (hAcomp: (a,b,A_SH) = AuSH.components5): Formula :=
-  Recreate8 (a, b, bForallTuple2 x t A_SH)
+  (hIntA: SH_int2 A AuSH) (hAcomp: (a,b,A_SH) = AuSH.components): Formula :=
+  Recreate (a, b, bForallTuple2 x t A_SH)
 
 def SH_int_bForall_comp (A : Formula) (x : List String) (t : List Term)
-  (hIntA: SH_int2 A AuSH) (hAcomp: (a,b,A_SH) = AuSH.components5): (List String × List String × Formula) :=
+  (hIntA: SH_int2 A AuSH) (hAcomp: (a,b,A_SH) = AuSH.components): (List String × List String × Formula) :=
   (a, b, bForallTuple2 x t A_SH)
 
 def SH_int_not_rec (A : Formula) {f a' : List String}
-  (hIntA: SH_int2 A AuSH) (hAcomp: (a,b,A_SH) = AuSH.components5): Formula :=
-  Recreate8 (f,a',(bForallTuple2 a (ls_lt a') (¬₁(A_SH.subst (HashMap.ofList  (b.zip ((f.tt)⊙(a.tt))))))))
+  (hIntA: SH_int2 A AuSH) (hAcomp: (a,b,A_SH) = AuSH.components): Formula :=
+  Recreate (f,a',(bForallTuple2 a (ls_lt a') (¬₁(A_SH.subst (HashMap.ofList  (b.zip ((f.tt)⊙(a.tt))))))))
+
+-- ---------------------------------------------------------
+
+-- EXAMPLE:
 
 open isAtomic
 open isBase
@@ -445,76 +336,33 @@ lemma lemazinho_testinho :
 #eval Testinho
 #check DoubleNeg Testinho
 
+-- ---------------------------------------------------------
+
+-- LEMMA: If A is base and A = B, then B must be base
+
+lemma baseEquality (A B:Formula) (hA : isBase A) (hEq : B = A) : isBase B := by
+  rw [hEq]
+  exact hA
+
+-- ---------------------------------------------------------
 
 -- Example: A ∨ (∀x∈t B)
-def baseBase (A:Formula) (hA : isBase A) (hIntA: SH_int2 A AuSH) (hAcomp: AuSH.components5 = ({},{},A_SH))
-  := A_SH = A
-
-lemma baseEquality (A B:Formula) (hA : isBase A) (hEq : B = A) : isBase B := by sorry
-
-example (A B : Formula) (hB : isBase B) (x:String) (t:Term)
-  (hIntA: SH_int2 A AuSH) (hAcomp: AuSH.components5 = (a,b,A_SH)) (hAcomp2: (a,b,A_SH) = AuSH.components5)
-  (hIntB: SH_int2 B BuSH) (hBcomp: BuSH.components5 = ({},{},B_SH)) (hBcomp2: ({},{},B_SH) = BuSH.components5)
-  (hIntEx : SH_int2 ( A ∨₁ (bForallTuple2 [x] [t] B) ) interp):
-  interp = Recreate8 (a,b, (A_SH ∨₁ (bForallTuple2 [x] [t] B))) :=
-by sorry
-  /-
-  --let H1 := SH_int_base_rec B hB
-  have H1simp : (SH_int_base_rec B hB) = (bForallTuple2 [x] [t] B) := by sorry
-  have H1comp : ({},{}, bForallTuple2 [x] [t] B) = (bForallTuple2 [x] [t] B).components5 := by sorry
-  have H1comp2 : (bForallTuple2 [x] [t] B).components5 = ({},{}, bForallTuple2 [x] [t] B) := by sorry
-  have Hcenas : B_SH = B := by sorry --exact (baseBase B hB hIntB hBcomp)
-  have HEq := (baseEquality B B_SH hB Hcenas)
-  have hSH := SH_int_bForall_comp B [x] [t] hIntB hBcomp2          -- Recreate8 ({}, {}, bForallTuple2 x t B)
-  have H := (@SH_int2.bForall B BuSH {} {} B_SH [x] t hIntB hBcomp HEq)
-  have Htwo : SH_int2 (bForallTuple2 [x] [t] B) (bForallTuple2 [x] [t] B)
-  have H2 : (Recreate2 (∅, ∅, bForallTuple2 [x] [t] B)).components5 = ({},{},bForallTuple2 [x] [t] B)
-  have HH {intAvB} : SH_int2 (bForallTuple2 [x] [t] B) intAvB
-  have Hcomp : SH_int2 (bForallTuple2 [x] [t] B) (Recreate2 (∅, ∅, b∀₁ [x] t B_SH))
-  sorry
-  --have Hcomp : (Recreate2 (∅, ∅, b∀₁ [x] t B_SH)).components5 = (∅, ∅, b∀₁ [x] t B_SH) := by sorry
-  --THIS have H3 := (@SH_int2.disj A AuSH (bForallTuple2 [x] [t] B) (Recreate2 (∅, ∅, b∀₁ [x] t B_SH)) a b A_SH {} {} (bForallTuple2 [x] [t] B) hIntA Hcomp)
-  -- have hSHtudo := SH_int_or_comp A (bForallTuple2 [x] [t] B) hIntA hAcomp
-  --have H2_simp : (SH_int_or_rec A B hIntA hAcomp hIntB hBcomp )
-  -/
-
-/-
-def SH_int_or_comp (A B : Formula)
-  (hIntA: SH_int2 A AuSH) (hAcomp: (a,b,A_SH) = AuSH.components5)
-  (hIntB: SH_int2 B BuSH) (hBcomp: (c,d,B_SH) = BuSH.components5): (List String × List String × Formula) :=
-  (a∪c, b∪d, (A_SH ∨₁ B_SH))
-
-  | bForall : SH_int2 A AuSH →
-            AuSH.components5 = (a,b,A_SH) →                                  -- A^SH = ∀a ∃b A_SH(a,b)
-            (hA : isBase A_SH) →
-            (SH_int2 (b∀₁ x t A) (Recreate2 (a,b,(b∀₁ x t A_SH))))
--/
-
-
 -- example (A:Formula) (hInt : SH_int2 A AuSH) → (hComp : (a,b,A_SH) = AuSH.components2) :
 
 example (A B:Formula) (H : SH_int2 (A→₁B) IMPuSH) {f a' :List String}:
-  (isBase A_SH) → (SH_int2 A AuSH) → ((a,b,A_SH) = AuSH.components2) →
-  (isBase B_SH) → (SH_int2 B BuSH) → ((c,d,B_SH) = AuSH.components2) →
-  ((IMPuSH.components2 = (f∪c,a'∪d,(A_SH →₁ B_SH)))) := by sorry
+  (isBase A_SH) → (SH_int2 A AuSH) → ((a,b,A_SH) = AuSH.components) →
+  (isBase B_SH) → (SH_int2 B BuSH) → ((c,d,B_SH) = AuSH.components) →
+  ((IMPuSH.components = (f∪c,a'∪d,(A_SH →₁ B_SH)))) := by sorry
 
 /-
-example (A B:Formula) (H : SH_int2 (A→₁B) IMPuSH) {f a' :List String}:
-  (isFullyBase A_SH) → (SH_int2 A AuSH) → ((a,b,A_SH) = AuSH.components2) →
-  (isFullyBase B_SH) → (SH_int2 B BuSH) → ((c,d,B_SH) = AuSH.components2) →
-  ((IMPuSH.components2 = (f∪c,a'∪d,(A_SH →₁ B_SH)))) :=
-  by
-    intro baseA
-    intro interpA
-    intro compA
-    intro baseB
-    intro interpB
-    intro compB
-    unfold F_implies
-    have HH := @SH_int2.neg A AuSH a b A_SH f a' interpA compA
-    sorry
+
 
 -- Vamos mostrar que se A^SH = ∀a ∃b A_SH e B^SH = ∀c B_SH que (A∨B)^SH = ∀a,c ∃b (A_SH ∨ B_SH)
+
+
+-- --------------------------------------------------------
+-- --------------------------------------------------------
+-- --------------------------------------------------------
 
 
 
@@ -533,20 +381,16 @@ def zz : List String := ["z"]
 def FormulaF : Formula := aaa =₁ bbb
 
 #check exAA xx yy FormulaF                 -- Formula ∀ "x"
-#check (exAA xx yy FormulaF).components2
-#eval (exAA xx yy FormulaF).components2
+#check (exAA xx yy FormulaF).components
+#eval (exAA xx yy FormulaF).components
 
 #eval (∀₁ ["x"] (∃₁ ["y"] (var "x" =₁ var "y")))              -- Formula ∀ "x" ∃ "y" (x=y)
-#eval (∀₁ ["x"] (∃₁ ["y"] (var "x" =₁ var "y"))).components2  -- no
-#eval (∀₁ ["x"] (∃₁ ["y"] (var "x" =₁ var "y"))).components5  -- yes
-#eval (∀₁ ["x"] (var "x" =₁ var "y")).components5  -- yes
-#eval (∃₁ ["y"] (var "x" =₁ var "y")).components5  -- yes
+#eval (∀₁ ["x"] (∃₁ ["y"] (var "x" =₁ var "y"))).components  -- yes
+#eval (∀₁ ["x"] (var "x" =₁ var "y")).components             -- yes
+#eval (∃₁ ["y"] (var "x" =₁ var "y")).components             -- yes
 
-def ThisTeste := (∀₁ ["x"] (∃₁ ["y"] (var "x" =₁ var "y"))).components2
-#eval Recreate2 ((∀₁ ["x"] (∃₁ ["y"] (var "x" =₁ var "y"))).components2)
-#eval Recreate2 ((∀₁ ["x"] (∃₁ ["y"] (var "x" =₁ var "y"))).components5)
-#eval Recreate5 ((∀₁ ["x"] (∃₁ ["y"] (var "x" =₁ var "y"))).components5)
-#eval Recreate7 ((∀₁ ["x"] (∃₁ ["y"] (var "x" =₁ var "y"))).components5)  -- yes
+#eval Recreate ((∀₁ ["x"] (∃₁ ["y"] (var "x" =₁ var "y"))).components)  -- yes
+#eval RecreateSimp ((∀₁ ["x"] (∃₁ ["y"] (var "x" =₁ var "y"))).components)  -- yes
 
 
 --theorem Soundness (A : Formula) (hA1 : SH_int2 A AuSH) (hA2 : AuSH.components2 = (a,b,A_SH)) (hA3 : isBase A_SH):
@@ -559,23 +403,28 @@ def ThisTeste := (∀₁ ["x"] (∃₁ ["y"] (var "x" =₁ var "y"))).components
         b) Axioms / FiniteTypes / Syntax / ResultsAndOtherDefinitions
     2. Resolver isBase como hipotese em components... done?
     3. Resolver Term.application para tuples -> Notation 1.4
-
-axiom Bla (A:Formula) : (¬₁(¬₁ A))=A
 -/
+
+
+
+-- --------------------------------------------------------
+-- --------------------------------------------------------
+-- --------------------------------------------------------
+
 
 
 -- mover
 open Axioms
 
-example : Formula.components2 (axiomE1 "x") = ([], [], (axiomE1 "x")) := by
+example : Formula.components (axiomE1_matrix "x") = ([], [], (axiomE1_matrix "x")) := by
   exact rfl
 
-example : (axiomE2 x₁ x₂ A hA).components2 = ([], [], (axiomE2 x₁ x₂ A hA)) := by sorry
+example : (axiomE2_matrix x₁ x₂ A hA).components = ([], [], (axiomE2_matrix x₁ x₂ A hA)) := by sorry
 
 
-#eval (axiomE1 "x").components2
+#eval (axiomE1_matrix "x").components
 -- Quero mostrar que pôr foralls antes dos axiomas, que não muda nada
 -- que SH_int2 de axiomE1 que é a mesma coisa que SH_int2 de AxiomE1
 --#eval
-#eval (AxiomE1 "x").components2
+#eval (AxiomE1 "x").components
 --#eval SH_int2 (AxiomE1 "x")
